theories/ml_toy_lang/adequacy.v
@@ -7,14 +7,14 @@ From iris.prelude Require Import options.
 
 Class heapGpreS Σ := HeapGpreS {
   heapGpreS_iris :> invGpreS Σ;
-  heapGpreS_heap :> gen_heapGpreS loc (option val) Σ;
-  heapGpreS_inv_heap :> inv_heapGpreS loc (option val) Σ;
+  heapGpreS_heap :> gen_heapGpreS loc val Σ;
+  heapGpreS_inv_heap :> inv_heapGpreS loc val Σ;
   heapGpreS_proph :> proph_mapGpreS proph_id (val * val) Σ;
   heapGS_step_cnt :> mono_natG Σ;
 }.
 
 Definition heapΣ : gFunctors :=
-  #[invΣ; gen_heapΣ loc (option val); inv_heapΣ loc (option val);
+  #[invΣ; gen_heapΣ loc val; inv_heapΣ loc val;
     proph_mapΣ proph_id (val * val); mono_natΣ].
 Global Instance subG_heapGpreS {Σ} : subG heapΣ Σ → heapGpreS Σ.
 Proof. solve_inG. Qed.
@@ -32,13 +32,13 @@ Proof.
   apply adequate_alt; intros t2 σ2 [n [κs ?]]%erased_steps_nsteps.
   eapply (wp_strong_adequacy Σ _); [|done].
   iIntros (Hinv).
-  iMod (gen_heap_init σ.(heap)) as (?) "[Hh _]".
-  iMod (inv_heap_init loc (option val)) as (?) ">Hi".
+  iMod (gen_heap_init σ) as (?) "[Hh _]".
+  iMod (inv_heap_init loc val) as (?) ">Hi".
   iMod (proph_map_init nil ∅) as (?) "Hp".
   iMod (mono_nat_own_alloc) as (γ) "[Hsteps _]".
   iDestruct (Hwp (HeapGS _ _ _ _ _ _ _ _) with "Hi") as "Hwp".
   iModIntro.
-  iExists (λ σ ns κs nt, (gen_heap_interp σ.(heap) ∗
+  iExists (λ σ ns κs nt, (gen_heap_interp σ ∗
                           mono_nat_auth_own γ 1 ns))%I.
   iExists [(λ v, ⌜φ v⌝%I)], (λ _, True)%I, _ => /=.
   iFrame.
