theories/ml_toy_lang/total_adequacy.v
@@ -10,13 +10,13 @@ Definition heap_total Σ {p:ml_program} `{!heapGpreS Σ} s e σ φ :
   sn erased_step ([e], σ).
 Proof.
   intros Hwp; eapply (twp_total _ _); iIntros (?) "".
-  iMod (gen_heap_init σ.(heap)) as (?) "[Hh _]".
-  iMod (inv_heap_init loc (option val)) as (?) ">Hi".
+  iMod (gen_heap_init σ) as (?) "[Hh _]".
+  iMod (inv_heap_init loc val) as (?) ">Hi".
   iMod (proph_map_init [] ∅) as (?) "Hp".
   iMod (mono_nat_own_alloc 0) as (γ) "[Hsteps _]".
   iModIntro.
   iExists
-    (λ σ ns κs _, (gen_heap_interp σ.(heap) ∗
+    (λ σ ns κs _, (gen_heap_interp σ ∗
                    mono_nat_auth_own γ 1 ns)%I),
     id, (λ _, True%I), _; iFrame.
   by iApply (Hwp (HeapGS _ _ _ _ _ _ _ _)).
